\documentclass[a4paper]{article}
\usepackage{enumitem}
\usepackage{tikz}
\usepackage{mathtools}
\usepackage{tabularx}
\input{head}
\input{formulas.tex}
\begin{document}

%-------------------------------
%   TITLE SECTION
%-------------------------------

\fancyhead[C]{}
\hrule \medskip % Upper rule
\begin{minipage}{0.295\textwidth}
    \raggedright
    \footnotesize
    Cor Zuurmond \hfill\\
    10580395 \hfill\\
    jczuurmond@gmail.com
\end{minipage}
\begin{minipage}{0.4\textwidth}
    \centering
    \large
    Homework Assignment 7\\
    \normalsize
    Machine Learning 2, 17/18\\
\end{minipage}
\begin{minipage}{0.295\textwidth}
    \raggedleft
    \today\hfill\\
\end{minipage}
\medskip\hrule
\bigskip

%-------------------------------
%   CONTENTS
%-------------------------------

\begin{align*}
    \label{eq:}
    D_{JL}(q(\vz) \parallel p(\vz)) & = \int q(\vz)
    \log\left(\frac{p(\vz)}{q(\vz)}\right) d\vz
    \\
    & = \int q(\vz) \log(p(\vz)) d\vz - \int q(\vz) \log(q(\vz)) d\vz 
    \\
    \int q(\vz) \log(p(\vz)) d\vz & = \int 
    q(\vz)
    \log\left(
    \frac{1}{\sqrt{(2\pi)^J \mid \mI \mid }}
    e^{-\frac{1}{2} \vz^T \mI^{-1} \vz)}
    \right) d\vz
    \\
    & = -\log\left(\sqrt{(2\pi)^J \mid \mI \mid } \right) + \int q(\vz)
    \left(-\frac{1}{2} \vz^T \mI^{-1} \vmu \right) d\vz 
    \\
    & = -\frac{J}{2} \log\left( 2\pi \right) - \frac{1}{2} \int
    \vz^T \vz q(\vz) d\vz
    \\
    & = -\frac{J}{2} \log\left( 2\pi \right) - \frac{1}{2} \int
    (\vz + \vmu)^T (\vz + \vmu) q(\vz + \vmu) d\vz
    \\
    & = -\frac{J}{2} \log\left( 2\pi \right) - \frac{1}{2} \int
    (\vz^T \vz + \vz^T \vmu + \vmu^T \vz + \vmu^T \vmu)
    q(\vz + \vmu) d\vz
    \\
    & = -\frac{J}{2} \log\left( 2\pi \right) - \frac{1}{2} \left(
    \EE{q(\vz + \vmu)}{\vz^T \vz} + \EE{q(\vz + \vmu)}{\vz^T \vmu} +
    \EE{q(\vz + \vmu)}{\vmu^T \vz} + \EE{q(\vz + \vmu)}{\vmu^T \vmu} \right)
    \\
    & = -\frac{J}{2} \log\left( 2\pi \right) - \frac{1}{2} \left(
    \trace{\diag{\vsigma} } + \trace{\vmu^T \vmu} \right)
    \\
    & = -\frac{J}{2} \log\left( 2\pi \right) - \frac{1}{2}
    \sumt{i=1}{J} \left( \vsigma_i^2 + \vmu_i^2 \right)
    \\
    \int q(\vz) \log(q(\vz)) d\vz & = \int 
    q(\vz)
    \log\left(
    \frac{1}{\sqrt{(2\pi)^J \mid \diag{\vsigma} \mid }}
    e^{-\frac{1}{2} (\vz - \vmu)^T (\diag{\vsigma} \cdot \diag{\vsigma})^{-1} (\vz - \vmu)}
    \right) d\vz
    \\ 
    & = -\frac{J}{2} \log\left( 2\pi \right) -
    \frac{J}{2} \log\left( \mid \diag{\vsigma} \cdot \diag{\vsigma} \mid \right) - \frac{1}{2} \int
    (\vz - \vmu)^T (\diag{\vsigma} \cdot \diag{\vsigma})^{-1} (\vz
    - \vmu) q(\vz) d\vz
    \\
    & = -\frac{J}{2} \log\left( 2\pi \right) -
    \frac{J}{2} \sumt{i=1}{J}(\log(\vsigma_i^2)) - \frac{1}{2} \int
    \vz^T (\diag{\vsigma} \cdot \diag{\vsigma})^{-1} \vz q(\vz + \vmu) d\vz
    \\
    & = -\frac{J}{2} \log\left( 2\pi \right) -
    \frac{J}{2} \sumt{i=1}{J}(\log(\vsigma_i^2)) - 
    \frac{1}{2} \EE{q(\vz + \vmu)}{\vz^T (\diag{\vsigma} \cdot
    \diag{\vsigma})^{-1} \vz} 
    \\
    & = -\frac{J}{2} \log\left( 2\pi \right) -
    \frac{J}{2} \sumt{i=1}{J}(\log(\vsigma_i^2)) - 
    \frac{1}{2} \trace{\EE{q(\vz + \vmu)}{\vz^T (\diag{\vsigma} \cdot
    \diag{\vsigma})^{-1} \vz} }
    \\
    & = -\frac{J}{2} \log\left( 2\pi \right) - 
    \frac{J}{2} \sumt{i=1}{J}(\log(\vsigma_i^2)) - \frac{1}{2}
    \trace{(\diag{\vsigma} \cdot \diag{\vsigma})^{-1} (\diag{\vsigma} \cdot
    \diag{\vsigma})}
    \\
    & = -\frac{J}{2} \log\left( 2\pi \right) - 
    \frac{J}{2} \sumt{i=1}{J}(\log(\vsigma_i^2)) - \frac{J}{2}
    \\
    & = -\frac{J}{2} \log\left( 2\pi \right) -
    \frac{J}{2} \sumt{i=1}{J} (\log(\vsigma_i^2) + 1)
    \\
    D_{JL}(q(\vz) \parallel p(\vz)) & = 
    \int q(\vz) \log(p(\vz)) d\vz - \int q(\vz) \log(q(\vz)) d\vz 
    \\
    & = -\frac{J}{2} \log\left( 2\pi \right) - \frac{1}{2}
    \sumt{i=1}{J} \left( \vsigma_i^2 + \vmu_i^2 \right)
    - \left(-\frac{J}{2} \log\left( 2\pi \right) -
    \frac{J}{2} \sumt{i=1}{J} (\log(\vsigma_i^2) + 1) \right)
    \\
    & = \frac{1}{2} \sumt{i=1}{J} \left( \log(\vsigma_i^2) + 1 - \vsigma_i^2 - \vmu_i^2\right)
\end{align*}


\end{document}
\grid
